dist/gcc-compatible/Hacl_AES_128_CTR32_NI.h
@@ -55,17 +55,12 @@ void Hacl_AES_128_CTR32_NI_context_free(Lib_IntVector_Intrinsics_vec128 *s);
 Initiate AES-128 context buffer with key expansion and nonce
 */
 void
-Hacl_AES_128_CTR32_NI_aes128_init(
-  Lib_IntVector_Intrinsics_vec128 *ctx,
-  uint8_t *key,
-  uint8_t *nonce
-);
+Hacl_AES_128_CTR32_NI_init(Lib_IntVector_Intrinsics_vec128 *ctx, uint8_t *key, uint8_t *nonce);
 
 /**
 Set nonce in AES-128 context buffer
 */
-void
-Hacl_AES_128_CTR32_NI_aes128_set_nonce(Lib_IntVector_Intrinsics_vec128 *ctx, uint8_t *nonce);
+void Hacl_AES_128_CTR32_NI_set_nonce(Lib_IntVector_Intrinsics_vec128 *ctx, uint8_t *nonce);
 
 /**
 Initiate AES-CTR32-128 context with key and nonce, and
@@ -75,7 +70,7 @@ Initiate AES-CTR32-128 context with key and nonce, and
   `counter` is the initial value of counter state.
 */
 void
-Hacl_AES_128_CTR32_NI_aes128_ctr_encrypt(
+Hacl_AES_128_CTR32_NI_ctr_encrypt(
   uint32_t len,
   uint8_t *out,
   uint8_t *inp,
@@ -94,7 +89,7 @@ Initiate AES-CTR32-128 context with key and nonce, and
   Decryption uses the forward version of AES cipher
 */
 void
-Hacl_AES_128_CTR32_NI_aes128_ctr_decrypt(
+Hacl_AES_128_CTR32_NI_ctr_decrypt(
   uint32_t len,
   uint8_t *out,
   uint8_t *inp,
