dist/gcc-compatible/lib/Hacl_AES_256_CTR32_NI_bindings.ml
@@ -2,15 +2,15 @@ open Ctypes
 module Bindings(F:Cstubs.FOREIGN) =
   struct
     open F
-    let hacl_AES_256_CTR32_NI_aes256_ctr_encrypt =
-      foreign "Hacl_AES_256_CTR32_NI_aes256_ctr_encrypt"
+    let hacl_AES_256_CTR32_NI_ctr_encrypt =
+      foreign "Hacl_AES_256_CTR32_NI_ctr_encrypt"
         (uint32_t @->
            (ocaml_bytes @->
               (ocaml_bytes @->
                  (ocaml_bytes @->
                     (ocaml_bytes @-> (uint32_t @-> (returning void)))))))
-    let hacl_AES_256_CTR32_NI_aes256_ctr_decrypt =
-      foreign "Hacl_AES_256_CTR32_NI_aes256_ctr_decrypt"
+    let hacl_AES_256_CTR32_NI_ctr_decrypt =
+      foreign "Hacl_AES_256_CTR32_NI_ctr_decrypt"
         (uint32_t @->
            (ocaml_bytes @->
               (ocaml_bytes @->
